src/Std/Data/DHashMap/Internal/WF.lean
@@ -479,9 +479,140 @@ theorem wfImp_insert [BEq α] [Hashable α] [EquivBEq α] [LawfulHashable α] {m
   rw [insert_eq_insertₘ]
   exact wfImp_insertₘ h
 
+theorem wfImp_modify [BEq α] [Hashable α] [LawfulBEq α] {m : Raw₀ α β}
+    (h : Raw.WFImp m.1) {a : α} {f : β a → β a} : Raw.WFImp (m.modify a f).1 := by
+  sorry
+
+/-! # `alter` -/
+
+theorem isHashSelf_alterₘ [BEq α] [Hashable α] [LawfulBEq α] (m : Raw₀ α β)
+    (h : Raw.WFImp m.1) (a : α) (f : Option (β a) → Option (β a)) : IsHashSelf (m.alterₘ a f).1.buckets := by
+  dsimp only [alterₘ]
+  split
+  · apply h.buckets_hash_self.updateBucket (fun l p hp => ?_)
+    rw [AssocList.toList_alter] at hp
+    induction l
+    · simp only [AssocList.alter] at hp
+      split at hp <;> try contradiction
+      simp only [AssocList.toList_cons, AssocList.toList_nil, mem_singleton] at hp
+      simp only [hp, AssocList.toList_nil, containsKey_nil, Bool.false_eq_true, or_true]
+    · next ih =>
+      simp only [AssocList.alter, beq_iff_eq] at hp
+      split at hp
+      · split at hp
+        · simp only [AssocList.toList_cons, containsKey_cons, Bool.or_eq_true, beq_iff_eq]
+          exact Or.inl <| Or.inr <| containsKey_of_mem hp
+        · simp only [AssocList.toList_cons, mem_cons] at hp
+          cases hp
+          · next h =>
+            simp only [h, AssocList.toList_cons, containsKey_cons, beq_self_eq_true, Bool.true_or,
+              true_or]
+          · next h =>
+            simp only [AssocList.toList_cons, containsKey_cons, Bool.or_eq_true, beq_iff_eq]
+            exact Or.inl <| Or.inr <| containsKey_of_mem h
+      · simp only [AssocList.toList_cons, mem_cons] at hp
+        cases hp
+        · next h =>
+          simp only [h, AssocList.toList_cons, containsKey_cons, beq_self_eq_true, Bool.true_or,
+            true_or]
+        · next h =>
+          simp only [AssocList.toList_cons, containsKey_cons, Bool.or_eq_true, beq_iff_eq]
+          cases ih h
+          · exact Or.inl <| Or.inr <| by assumption
+          · exact Or.inr <| by assumption
+  · split
+    · exact h.buckets_hash_self
+    · refine (wfImp_expandIfNecessary _ ?_).buckets_hash_self
+      apply wfImp_consₘ <;> { simp only [Bool.not_eq_true] at *; assumption }
+
+theorem toListModel_alterₘ [BEq α] [Hashable α] [LawfulBEq α] {m : Raw₀ α β} (h : Raw.WFImp m.1) {a : α}
+    {f : Option (β a) → Option (β a)} :
+    Perm (toListModel (m.alterₘ a f).1.2) (alterKey a f (toListModel m.1.2)) := by
+  rw [alterₘ]
+  split
+  · dsimp only [AssocList.contains_eq, bucket_updateBucket]
+    refine toListModel_updateBucket h ?_ ?_ ?_
+    · exact AssocList.toList_alter
+    · exact List.alterKey_of_perm
+    · exact List.alterKey_append_of_containsKey_right_eq_false
+  · next hc =>
+    simp only [Bool.not_eq_true] at hc
+    rw [alterKey, getValueCast?_eq_none (by simpa only [← containsₘ_eq_containsKey h] using hc)]
+    split
+    · next hn =>
+      simp only [hn]
+      rw [eraseKey_of_containsKey_eq_false]
+      simpa only [← containsₘ_eq_containsKey h] using hc
+    · next hs =>
+      simp only [hs]
+      refine Perm.trans (toListModel_expandIfNecessary _) ?_
+      refine Perm.trans (toListModel_consₘ m h _ _) ?_
+      rw [insertEntry_of_containsKey_eq_false]
+      simpa only [← containsₘ_eq_containsKey h] using hc
+
+theorem containsₘ_alter_iff [BEq α] [Hashable α] [LawfulBEq α] {m : Raw₀ α β} (h : Raw.WFImp m.1)
+    {a : α} {f : Option (β a) → Option (β a)} :
+    (m.alter a f).containsₘ a ↔ (f (m.get?ₘ a)).isSome := by
+  simp only [alter_eq_alterₘ, alterₘ, Array.uset, Array.set_set]
+  if hc : m.containsₘ a then
+    have hc₁ := containsₘ_eq_containsKey h ▸ hc
+    -- rw [get?_eq_getValueCast?, getValueCast?_eq_some_getValueCast hc₁]
+    have hc₂ := hc
+    simp only [hc₂, reduceIte, AssocList.contains_eq]
+    simp only [containsₘ, reduceDIte, bucket_updateBucket, AssocList.contains_eq]
+    simp only [AssocList.toList_alter]
+    rw [containsKey_alterKey_iff]
+    -- rw [get?_eq_getValueCast?, getValueCast?_eq_some_getValueCast]
+    rw [get?ₘ]
+    simp?
+    · have := h.distinct
+      rw [toListModel] at this
+    done
+  else
+    done
+
+theorem bucket_alter [BEq α] [Hashable α] [LawfulBEq α] {m : Raw₀ α β} (h : Raw.WFImp m.1)
+    {a : α} {f : Option (β a) → Option (β a)} :
+    bucket (m.alter a f).1.buckets (m.alter a f).2 a = (bucket m.1.buckets m.2 a).alter a f := sorry
+
+/-- Internal implementation detail of the hash map -/
+theorem wfImp_alterₘ [BEq α] [Hashable α] [LawfulBEq α] {m : Raw₀ α β} (h : Raw.WFImp m.1) {a : α}
+    {f : Option (β a) → Option (β a)} :
+    Raw.WFImp (m.alterₘ a f).1 where
+  buckets_hash_self := isHashSelf_alterₘ m h a f
+  size_eq := by
+    refine Eq.trans ?_ (Perm.length_eq (toListModel_alterₘ h).symm)
+    rw [alterₘ]
+    split
+    · next hc =>
+      rw [containsₘ_eq_containsKey h] at hc
+      have : (m.alter a f).containsₘ a ↔ _ := containsₘ_alter_iff h
+      rw [containsₘ, bucket_alter h] at this
+      simp only [bucket_updateBucket, this, get?_eq_getValueCast? h, alterKey]
+      apply Eq.symm; split <;> { next hh =>
+        simp [length_insertEntry, length_eraseKey, hc, hh, h.size_eq] }
+    · next hc =>
+      simp only [containsₘ_eq_containsKey h, Bool.not_eq_true] at hc
+      simp only [alterKey]
+      rw [getValueCast?_eq_none hc]
+      split
+      · next heq =>
+        simp only [h.size_eq, heq, length_eraseKey, hc, Bool.false_eq_true, reduceIte]
+      · next heq =>
+        simp only [heq, length_insertEntry, hc, Bool.false_eq_true, reduceIte]
+        rw [(wfImp_expandIfNecessary _
+          (wfImp_consₘ _ h _ _ (by simpa [containsₘ_eq_containsKey h] using hc))).size_eq]
+        rw [(toListModel_expandIfNecessary _).length_eq, (toListModel_consₘ _ h _ _).length_eq,
+          length_cons]
+  distinct := by
+    apply DistinctKeys.perm <| toListModel_alterₘ h
+    apply distinctKeys_alterKey
+    exact h.distinct
+
 theorem wfImp_alter [BEq α] [Hashable α] [LawfulBEq α] {m : Raw₀ α β}
     (h : Raw.WFImp m.1) {a : α} {f : Option (β a) → Option (β a)} : Raw.WFImp (m.alter a f).1 := by
-  sorry
+  rw [alter_eq_alterₘ]
+  exact wfImp_alterₘ h
 
 /-! # `containsThenInsert` -/
 
@@ -751,6 +882,7 @@ theorem WF.out [BEq α] [Hashable α] [i₁ : EquivBEq α] [i₂ : LawfulHashabl
   · next h => exact Raw₀.wfImp_getThenInsertIfNew? (by apply h)
   · next h => exact Raw₀.wfImp_filter (by apply h)
   · next h => exact Raw₀.Const.wfImp_getThenInsertIfNew? (by apply h)
+  · next h => exact Raw₀.wfImp_modify (by apply h)
   · next h => exact Raw₀.wfImp_alter (by apply h)
 
 end Raw
